wip: refund refund

crowdfunding.v
@@ -141,10 +141,16 @@ Definition crowdfunding : full_contract false parameter_ty None storage_ty :=
       {NIL operation; SWAP; CONS; PAIR})}}}.
 
 Local Definition geq a b :=
-  BinInt.Z.compare a b = Gt \/ BinInt.Z.compare a b = Eq.
+  match BinInt.Z.compare a b with
+  | Gt | Eq => true
+  | _ => false
+  end.
 
 Local Definition gt a b :=
-  BinInt.Z.compare a b = Gt.
+  match BinInt.Z.compare a b with
+  | Gt => true
+  | _ => false
+  end.
 
 Import Notations.
 
@@ -213,6 +219,30 @@ Proof.
       (try by move=> + []).
 Qed.
 
+Lemma crowdfunding_fail_contribute
+      (env : @proto_env (Some (parameter_ty, None)))
+      (fuel : Datatypes.nat)
+      (refund_address : data key_hash)
+      (raisers : data (set address))
+      (refund_table : data (big_map address mutez))
+      (funding_start : data timestamp)
+      (funding_end : data timestamp)
+      (unconditional_refund_start : data timestamp)
+      (withdrawn : data bool) :
+fuel <= 5 ->
+~~ success (eval_seq env crowdfunding fuel
+         (inl refund_address,
+          ((raisers, refund_table),
+           ((withdrawn, funding_start),
+            (funding_end, unconditional_refund_start))), tt)).
+Proof.
+  case: fuel => //.
+  repeat case => //.
+  rewrite /eval_seq /=.
+  case: (map.get _ _ _ _ ) => // a.
+  case: (tez.of_Z _) => //.
+Qed.
+
 Lemma crowdfunding_correct_withdraw
       (env : @proto_env (Some (parameter_ty, None)))
       (fuel : Datatypes.nat)
@@ -249,10 +279,31 @@ Proof.
     case: (BinInt.Z.compare (now env) unconditional_refund_start) => // + + a *;
     repeat split => //; auto; by move/negP/negP: a).
   + case=> + [] + [] + [] + [].
-    case: (BinInt.Z.compare (now env) funding_start) => //;
-    case: (BinInt.Z.compare funding_end (now env)) => //;
-    case=> [] // ? [] // ? -> ? a *;
+    case: (BinInt.Z.compare (now env) funding_start) => // _;
+    case: (BinInt.Z.compare funding_end (now env)) => // _;
+    case: (BinInt.Z.compare unconditional_refund_start (now env)) => // _ *;
     repeat split => //; auto; by apply/negP/negP.
+Qed.
+
+Lemma crowdfunding_fail_withdraw
+      (env : @proto_env (Some (parameter_ty, None)))
+      (fuel : Datatypes.nat)
+      (beneficiary : data address)
+      (raisers : data (set address))
+      (refund_table : data (big_map address mutez))
+      (funding_start : data timestamp)
+      (funding_end : data timestamp)
+      (unconditional_refund_start : data timestamp)
+      (withdrawn : data bool) :
+fuel <= 7 ->
+~~ success (eval_seq env crowdfunding fuel
+         (inr (inl beneficiary),
+          ((raisers, refund_table),
+           ((withdrawn, funding_start),
+            (funding_end, unconditional_refund_start))), tt)).
+Proof.
+  case: fuel => //.
+  repeat case => //.
 Qed.
 
 Lemma crowdfunding_correct_refund
@@ -294,6 +345,29 @@ Proof.
     repeat split; auto.
     rewrite /= BinInt.Z.compare_antisym.
     by case: H2; case: (BinInt.Z.compare (now env) unconditional_refund_start); auto.
+Qed.
+
+Lemma crowdfunding_fail_refund
+      (env : @proto_env (Some (parameter_ty, None)))
+      (fuel : Datatypes.nat)
+      (eligible_address : data address)
+      (raisers : data (set address))
+      (refund_table : data (big_map address mutez))
+      (funding_start : data timestamp)
+      (funding_end : data timestamp)
+      (unconditional_refund_start : data timestamp)
+      (withdrawn : data bool) :
+fuel <= 7 ->
+~~ success (eval_seq env crowdfunding fuel
+         (inr (inr eligible_address),
+          ((raisers, refund_table),
+           ((withdrawn, funding_start),
+            (funding_end, unconditional_refund_start))), tt)).
+Proof.
+  case: fuel => //.
+  repeat case => //;
+  rewrite /eval_seq /=;
+  case: (map.get _ _ _ _ ) => //.
 Qed.
 
 (* 90 days = (60*60*24*90) seconds *)
@@ -359,4 +433,650 @@ Definition validation_snippet :
 
 Definition crowdfunding_genprog_validation_snippet :=
   make_typed_validation_snippet validation_snippet.
+
+Hypothesis new_env :
+  forall {N : self_info},
+    @proto_env N -> data (list operation) -> @proto_env N.
+
+Section Composition.
+Definition comp {tffB T U}
+           (N : self_info)
+           (env : @proto_env N)
+           (A : stack (pair (list operation) U ::: [::]))
+           (paramB : data T)
+           fuelB
+           (B : instruction_seq N tffB (pair T U :: [::])
+                                (pair (list operation) U :: [::])) :=
+  let '(opsA, storage, tt) := A in
+  match eval_seq env B fuelB (paramB, storage, tt) with
+  | Return (opsB, storage, tt) =>
+    (new_env env opsB, (cat opsA opsB, storage, tt))
+  | Failed _ =>
+    (env, (opsA, storage, tt))
+  end.
+
+Definition compN {tff T U N}
+           (I : instruction_seq N tff (pair T U :: [::])
+                                (pair (list operation) U :: [::]))
+           xs env storage :=
+  foldr (fun b a => comp a.1 a.2 b.1 b.2 I) (env, ([::], storage, tt)) xs.
+End Composition.
+
+Inductive Operation :=
+| TransferTokens : forall
+    (env : @proto_env (Some (parameter_ty, None)))
+    (m : tez.mutez)
+    (d : data (contract unit)), Operation.
+
+Definition eval_seq_another
+      (env : @proto_env (Some (parameter_ty, None)))
+      (fuel : Datatypes.nat)
+      (A : stack (pair parameter_ty storage_ty ::: [::])) :=
+  let refund_amount x := map.get _ _ _
+                             (address_ _ (implicit_account x)) in
+  let remove := map.remove address_constant tez.mutez address_compare
+              (compare_eq_iff address) (lt_trans address) (gt_trans address) in
+  let get := map.get address_constant tez.mutez address_compare in
+  let '((raisers, refund_table),
+           ((withdrawn, funding_start),
+            (funding_end, unconditional_refund_start))) := A.1.2 in
+  match A.1.1 with
+  | inr (inr eligible_address) =>
+    match get eligible_address refund_table with
+    | Some y =>
+      match contract_ None unit eligible_address with
+      | Some y0 =>
+        if (7 < fuel) && geq (now env) unconditional_refund_start && (withdrawn == false)
+        then Return ([:: TransferTokens env y y0],
+                (raisers, remove eligible_address refund_table,
+                 (withdrawn, funding_start, (funding_end, unconditional_refund_start))), tt)
+        else Failed _ Overflow
+      | None => Failed _ Overflow
+      end
+    | None => Failed _ Overflow
+    end
+  | inr (inl beneficiary) =>
+    match contract_ None unit beneficiary with
+    | None => Failed _ Overflow
+    | Some y =>
+      if (7 < fuel) && geq (now env) funding_start && geq funding_end (now env)
+         && gt unconditional_refund_start (now env)
+         && (set.mem address_constant address_compare (source env) raisers)
+         && (withdrawn == false)
+      then Return ([:: TransferTokens env (balance env) y],
+          (raisers, refund_table,
+          (true, funding_start, (funding_end, unconditional_refund_start))), tt)
+      else Failed _ Overflow
+    end
+  | inl refund_address =>
+    let insert := map.insert address_constant tez.mutez address_compare
+                     (compare_eq_iff address) (gt_trans address)
+                     (Implicit refund_address) in
+    let! t :=
+        match refund_amount refund_address refund_table with
+        | Some x =>
+          let! z := tez.of_Z (BinInt.Z.add (tez.to_Z (amount env)) (tez.to_Z x)) in
+          Return (insert z refund_table)
+        | None =>
+          Return (insert (amount env) refund_table)
+        end in
+    if (5 < fuel) && geq (now env) funding_start && geq funding_end (now env)
+    then Return ([::],
+            ((raisers, t),
+             ((withdrawn, funding_start),
+              (funding_end, unconditional_refund_start))), tt)
+    else Failed _ Overflow
+  end.
+
+Local Definition conv (o : Operation) :=
+  match o with
+  | TransferTokens env m d =>
+    transfer_tokens env unit tt m d
+  end.
+
+Local Definition destination (o : Operation) :=
+  match o with
+  | TransferTokens env m d => d
+  end.
+
+Lemma eval_seq_eq env fuel A :
+  success (eval_seq env crowdfunding fuel A) ->
+  eval_seq env crowdfunding fuel A =
+  let! (ops, storage, tt) := eval_seq_another env fuel A in
+  Return (seq.map conv ops, storage, tt).
+Proof.
+  case: A => [][] op st [].
+  case: st => [][] raisers refund_table [][] withdrawn funding_start
+              [] funding_end unconditional_refund_start.
+  case: op => [refund_address|[beneficiary|eligible_address]] s.
+  + have f5 : 5 < fuel.
+     rewrite ltnNge.
+     apply/negP => /(crowdfunding_fail_contribute
+     env refund_address raisers refund_table funding_start funding_end unconditional_refund_start withdrawn).
+     by rewrite s.
+    have: is_true (success (eval_seq env crowdfunding fuel (inl refund_address, (raisers, refund_table, (withdrawn, funding_start, (funding_end, unconditional_refund_start))), tt)))
+     by rewrite s.
+    rewrite success_precond crowdfunding_correct_contribute //= /eval_seq_another /=.
+    set B := match _ with | Some _ => _ | None => _ end .
+    case Beq : B => //= [][] Ha [] Hb _.
+    rewrite Ha Hb f5 return_precond crowdfunding_correct_contribute //.
+    subst B; rewrite Beq /=.
+    by auto.
+  + have f7 : 7 < fuel.
+     rewrite ltnNge.
+     apply/negP => /(crowdfunding_fail_withdraw
+     env beneficiary raisers refund_table funding_start funding_end unconditional_refund_start withdrawn).
+     by rewrite s.
+    have: is_true (success (eval_seq env crowdfunding fuel (inr (inl beneficiary), (raisers, refund_table, (withdrawn, funding_start, (funding_end, unconditional_refund_start))), tt)))
+     by rewrite s.
+    rewrite success_precond crowdfunding_correct_withdraw //= /eval_seq_another /=.
+    case=> []a1 []a2 []a3 []a4 []a5 []y [] Hy _.
+    rewrite a1 a2 a3 a4 a5 f7 Hy return_precond crowdfunding_correct_withdraw //.
+    repeat split => //.
+    by exists y; auto.
+  + have f7 : 7 < fuel.
+     rewrite ltnNge.
+     apply/negP => /(crowdfunding_fail_refund
+     env eligible_address raisers refund_table funding_start funding_end unconditional_refund_start withdrawn).
+     by rewrite s.
+    have: is_true (success (eval_seq env crowdfunding fuel (inr (inr eligible_address), (raisers, refund_table, (withdrawn, funding_start, (funding_end, unconditional_refund_start))), tt)))
+     by rewrite s.
+    rewrite success_precond crowdfunding_correct_refund //= /eval_seq_another /=.
+    case=> []y []Hy []a1 []a2 []y0 []Hy0 _.
+    rewrite Hy Hy0 a1 a2 f7 return_precond crowdfunding_correct_refund //.
+    exists y; repeat split => //.
+    exists y0; by auto.
+Qed.
+
+Lemma eval_seq_fail env fuel A :
+  ~~ success (eval_seq env crowdfunding fuel A) <->
+  ~~ success (eval_seq_another env fuel A).
+Proof.
+  case: A => [][] op st [].
+  case: st => [][] raisers refund_table [][] withdrawn funding_start
+              [] funding_end unconditional_refund_start.
+  case: op => [refund_address|[beneficiary|eligible_address]];
+  split; apply/contra => s.
+  + apply/Bool.Is_true_eq_true.
+    rewrite -/Is_true -/is_true success_precond.
+    have f5: 5 < fuel.
+     rewrite ltnNge.
+     apply/negP => f5.
+     move: s.
+     rewrite /eval_seq_another /= ltnNge f5 /=.
+     by case: (match _ with | Some _ => _ | None => _ end).
+    rewrite crowdfunding_correct_contribute //=.
+    move: s.
+    rewrite /eval_seq_another /=.
+    set B := (match _ with | Some _ => _ | None => _ end).
+    case Beq : B => //.
+    rewrite f5 /=.
+    case: (geq (now env) funding_start) => //.
+    by case: (geq funding_end (now env)).
+  + apply/Bool.Is_true_eq_true.
+    rewrite -/Is_true -/is_true success_precond.
+    have f5: 5 < fuel.
+     rewrite ltnNge.
+     apply/negP => /(crowdfunding_fail_contribute
+     env refund_address raisers refund_table funding_start funding_end unconditional_refund_start withdrawn).
+     by rewrite s.
+    rewrite /eval_seq_another /= f5 /=.
+    move/Bool.Is_true_eq_left: s.
+    rewrite -/Is_true -/is_true success_precond crowdfunding_correct_contribute //=.
+    set B := (match _ with | Some _ => _ | None => _ end).
+    case Beq : B => //=.
+    case: (geq (now env) funding_start) => [|[]//].
+    by case: (geq funding_end (now env)) => [|[] _ []].
+  + apply/Bool.Is_true_eq_true.
+    rewrite -/Is_true -/is_true success_precond.
+    have f7: 7 < fuel.
+     rewrite ltnNge.
+     apply/negP => f7.
+     move: s.
+     rewrite /eval_seq_another /= ltnNge f7 /=.
+     by case: (contract_ None unit beneficiary).
+    rewrite crowdfunding_correct_withdraw //=.
+    move: s.
+    rewrite /eval_seq_another /=.
+    case Ceq: (contract_ _ _ _) => [a|//].
+    rewrite f7 /=.
+    case: (geq (now env) funding_start) => //.
+    case: (geq funding_end (now env)) => //.
+    case: (gt unconditional_refund_start (now env)) => //.
+    case: (set.mem address_constant address_compare (source env) raisers) => //.
+    case: withdrawn => //= _.
+    repeat split => //.
+    by exists a.
+  + apply/Bool.Is_true_eq_true.
+    rewrite -/Is_true -/is_true success_precond.
+    have f7: 7 < fuel.
+     rewrite ltnNge.
+     apply/negP => /(crowdfunding_fail_withdraw
+     env beneficiary raisers refund_table funding_start funding_end unconditional_refund_start withdrawn).
+     by rewrite s.
+    rewrite /eval_seq_another /= f7 /=.
+    move/Bool.Is_true_eq_left: s.
+    rewrite -/Is_true -/is_true success_precond crowdfunding_correct_withdraw //=.
+    by case=> []-> []-> []-> []-> []-> []y []-> _ /=.
+  + apply/Bool.Is_true_eq_true.
+    rewrite -/Is_true -/is_true success_precond.
+    have f7: 7 < fuel.
+     rewrite ltnNge.
+     apply/negP => f7.
+     move: s.
+     rewrite /eval_seq_another /= ltnNge f7 /=.
+     case: (map.get  _ _ _ _ _) => //.
+     by case: (contract_ _ _ _).
+    rewrite crowdfunding_correct_refund //=.
+    move: s.
+    rewrite /eval_seq_another /= f7 /=.
+    case Teq: (map.get  _ _ _ _ _) => [t|//].
+    case Ceq: (contract_ _ _ _) => [a|//].
+    case: (geq (now env) unconditional_refund_start) => //.
+    case: withdrawn => //= _.
+    exists t; repeat split => //.
+    by exists a.
+  + apply/Bool.Is_true_eq_true.
+    rewrite -/Is_true -/is_true success_precond.
+    have f7: 7 < fuel.
+     rewrite ltnNge.
+     apply/negP => /(crowdfunding_fail_refund
+     env eligible_address raisers refund_table funding_start funding_end unconditional_refund_start withdrawn).
+     by rewrite s.
+    rewrite /eval_seq_another /= f7 /=.
+    move/Bool.Is_true_eq_left: s.
+    rewrite -/Is_true -/is_true success_precond crowdfunding_correct_refund //=.
+    by case=> []x []-> []-> []-> []x0 []-> _.
+Qed.
+
+Definition comp_another
+           (env : @proto_env (Some (parameter_ty, None)))
+           (A : seq Operation * data storage_ty * Datatypes.unit)
+           (paramB : data parameter_ty)
+           fuelB :=
+  let '(opsA, storage, tt) := A in
+  match eval_seq_another env fuelB (paramB, storage, tt) with
+  | Return (opsB, storage, tt) =>
+    (new_env env (seq.map conv opsB), (cat opsA opsB, storage, tt))
+  | Failed _ =>
+    (env, (opsA, storage, tt))
+  end.
+
+Definition compN_another xs env storage :=
+  foldr (fun b a => comp_another a.1 a.2 b.1 b.2) (env, ([::], storage, tt)) xs.
+
+Lemma comp_eq env ops st paramB fuelB :
+  comp env (seq.map conv ops, st, tt) paramB fuelB crowdfunding
+= let '(env, (ops, st, tt)) := comp_another env (ops, st, tt) paramB fuelB in
+  (env, (seq.map conv ops, st, tt)).
+Proof.
+  rewrite /comp /comp_another.
+  set A := eval_seq_another _ _ _.
+  case Aeq : A => [|a].
+   have/eval_seq_fail: ~~ success A by rewrite Aeq.
+   by case: (eval_seq env crowdfunding fuelB (paramB, st, tt)).
+  set C := eval_seq env crowdfunding fuelB (paramB, st, tt).
+  have/eval_seq_eq: success C.
+   apply/negP => /negP /eval_seq_fail.
+   by subst A; rewrite Aeq.
+  subst C => ->.
+  subst A; rewrite Aeq.
+  case: a Aeq => [][] opsA st0 [] /= ?.
+  by rewrite map_cat.
+Qed.
+
+Lemma compN_eq env xs storage :
+  compN crowdfunding xs env storage
+= let '(env, (ops, st, tt)) := compN_another xs env storage in
+  (env, (seq.map conv ops, st, tt)).
+Proof.
+  elim: xs env storage => // x xs IH env storage.
+  rewrite /= !IH //=.
+  case: (compN_another xs env storage) => [] env0 [][] ops st [].
+  case s: (success (eval_seq env0 crowdfunding x.2 (x.1, st, tt))).
+  + rewrite /= eval_seq_eq //.
+    case: (eval_seq_another env0 x.2 (x.1, st, tt)) => [//|] [][]? ? [].
+    by rewrite map_cat.
+  + have: ~~ success (eval_seq_another env0 x.2 (x.1, st, tt))
+     by rewrite -eval_seq_fail s.
+    move: s => /=.
+    case: (eval_seq env0 crowdfunding x.2 (x.1, st, tt)) => //.
+    by case: (eval_seq_another env0 x.2 (x.1, st, tt)).
+Qed.
+
+Definition address_constant_eq a b :=
+  match a, b with
+  | Implicit (Mk_key_hash x), Implicit (Mk_key_hash y) => eqb x y
+  | Originated (Mk_smart_contract_address x),
+    Originated (Mk_smart_contract_address y) => eqb x y
+  | _, _ => false
+  end.
+
+Lemma comparable_data_eqP :
+  Equality.axiom (address_constant_eq).
+Proof.
+  case=> [][]x [][]y; apply/(iffP idP) => //= [];
+  (try by move/eqb_spec => ->);
+  by case=> ->; apply/eqb_spec.
+Qed.
+
+Canonical comparable_data_eqMixin := EqMixin comparable_data_eqP.
+Canonical comparable_data_eqType :=
+  Eval hnf in EqType _ comparable_data_eqMixin.
+
+Definition operation_constant_eq a b :=
+  match a, b with
+  | Mk_operation x, Mk_operation y => eqb x y
+  end.
+
+Lemma operation_constant_eqP :
+  Equality.axiom operation_constant_eq.
+Proof.
+  case=> []x []y; apply/(iffP idP) => /= [/eqb_spec -> //|[]->].
+  by apply/eqb_spec.
+Qed.
+
+Canonical operation_constant_eqMixin := EqMixin operation_constant_eqP.
+Canonical operation_constant_eqType :=
+  Eval hnf in EqType (data operation) operation_constant_eqMixin.
+
+Lemma refund_refund
+      (xs : seq (data parameter_ty * Datatypes.nat))
+      storage :
+let '(env, (ops, storage, tt)) := compN_another env xs storage in
+@uniq [eqType of data operation] (seq.map (transfer_tokens_proj3_morph transfer_tokens_proj3) res.1).
+
+Definition collect_eligible_address (xs : seq (data parameter_ty * Datatypes.nat))
+  := undup (foldl cat [::] (seq.map (fun x => match x.1 with
+                                   | inr (inr y) => [:: y]
+                                   | _ => [::]
+                                   end) xs)).
+
+Definition enough_fuel (a : data parameter_ty * Datatypes.nat) :=
+  match a.1 with
+  | inr (inr _) | inr (inl _) => a.2 > 7
+  | inl _ => a.2 > 5
+  end.
+Lemma size_crowdfunding_operations env x y z a b:
+  eval_seq env crowdfunding x (y, z, tt) = Return (a, b, tt) ->
+  seq.size a <= 1.
+Proof.
+  rewrite return_precond.
+  case: z => [][] raisers refund_table [][] withdrawn funding_start
+              [] funding_end unconditional_refund_start.
+  case: y => [|[]] y H; move: (H).
+  + rewrite crowdfunding_correct_contribute.
+     case: (map.get _ _ _ _ ) => /= [?|[]?[]?[]<- //].
+     case: (tez.of_Z _) => //= ?[]?[]?[]<- //.
+    rewrite leqNgt; apply/negP => C.
+    move: H (crowdfunding_fail_contribute env y raisers refund_table funding_start funding_end unconditional_refund_start withdrawn (eq^~ (a, b, tt)) C).
+    by rewrite -return_precond => ->.
+  + rewrite crowdfunding_correct_withdraw.
+     by case=> []?[]?[]?[]?[]?[]?[]?[]<-.
+    rewrite leqNgt; apply/negP => C.
+    move: H (crowdfunding_fail_withdraw env y raisers refund_table funding_start funding_end unconditional_refund_start withdrawn (eq^~ (a, b, tt)) C).
+    by rewrite -return_precond => ->.
+  + rewrite crowdfunding_correct_refund.
+     by case=> []?[]?[]?[]?[]?[]?[]<-.
+    rewrite leqNgt; apply/negP => C.
+    move: H (crowdfunding_fail_refund env y raisers refund_table funding_start funding_end unconditional_refund_start withdrawn (eq^~ (a, b, tt)) C).
+    by rewrite -return_precond => ->.
+Qed.
+
+Definition pre refund_table
+           (xs : seq (data parameter_ty * (Datatypes.nat * (@proto_env (Some (parameter_ty, None)))))) :=
+  let get := map.get address_constant tez.mutez address_compare in
+  seq.map (fun x => match x.1 with
+                 | inr (inr y) =>
+                   match get y refund_table, contract_ None unit y with
+                   | Some w, Some z =>
+                     (* x.2.2 *)
+                     Some (transfer_tokens x.2.2 unit tt w z)
+                   | _, _ => None
+                   end
+                 | inr (inl y) =>
+                   match contract_ None unit y with
+                   | Some z =>
+                     Some (transfer_tokens x.2.2 unit tt (balance x.2.2) z)
+                   | _ => None
+                   end
+                 | inl y => None
+                 end) xs.
+
+Definition prefold t xs :=
+  foldr (fun x y => match x with
+                 | Some z => z :: y
+                 | None => y
+                 end) [::] (pre t xs).
+
+Lemma prefold_cons t x xs :
+  let get := map.get address_constant tez.mutez address_compare in
+  prefold t (x :: xs) =
+  match
+  match x.1 with
+  | inr (inr y) =>
+    match get y t, contract_ None unit y with
+    | Some w, Some z =>
+      Some (transfer_tokens x.2.2 unit tt w z)
+    | _, _ => None
+    end
+  | inr (inl y) =>
+    match contract_ None unit y with
+    | Some z =>
+      Some (transfer_tokens x.2.2 unit tt (balance x.2.2) z)
+    | _ => None
+    end
+  | inl y => None
+  end
+  with
+  | None => prefold t xs
+  | Some y => y :: prefold t xs
+  end.
+Proof. by []. Qed.
+
+Lemma compN_operations xs storage :
+(compN crowdfunding xs storage).1.1 = prefold storage.1.2 xs.
+Proof.
+  elim: xs storage => //= x xs IH.
+  case => [][] raisers refund_table [][] withdrawn funding_start
+           [] funding_end unconditional_refund_start.
+  rewrite /= prefold_cons.
+  case: x => x1 [] x2 x3.
+  case: x1 => [|[]] x1.
+  + rewrite /comp /=.
+    move eq: (eval_seq _ _ _ _) => B.
+    case: B eq => [??|]; first by apply/IH.
+    case=> [][] a storage [] /=.
+    rewrite IH /= return_precond.
+    case x5 : (x2 > 5); last first.
+     move/negP/negP: x5; rewrite -leqNgt => C.
+     case: (compN crowdfunding xs (raisers, refund_table, (withdrawn, funding_start, (funding_end, unconditional_refund_start)))).1.2.
+     move=> [] raisers' refund_table' [][] withdrawn' funding_start'
+           [] funding_end' unconditional_refund_start' H.
+     move: H (crowdfunding_fail_contribute x3 x1 raisers' refund_table' funding_start' funding_end' unconditional_refund_start' withdrawn' (eq^~ (a, storage, tt)) C).
+     by rewrite -return_precond => ->.
+    case: (compN crowdfunding xs (raisers, refund_table, (withdrawn, funding_start, (funding_end, unconditional_refund_start)))).1.2.
+    move=> [] raisers' refund_table' [][] withdrawn' funding_start'
+          [] funding_end' unconditional_refund_start'.
+    rewrite crowdfunding_correct_contribute //=.
+    case: (map.get _ _ _ _ _) => [?|].
+     by case: (tez.of_Z _) => [] //= ? []?[]? []<-.
+    by case: (tez.of_Z _) => [] //= ? []?[]? []<-.
+  + rewrite /comp /=.
+    move eq: (eval_seq _ _ _ _) => B.
+    case: B eq => [? eq|].
+     rewrite IH.
+     rewrite /=.
+    first by apply/IH.
+     rewrite /=.
+    rewrite
+
+    rewrite /=.
+  rewrite /prefold /pre /=.
+  rewrite /=.
+  rewrite /=.
+
+Variable (env : @proto_env (Some (parameter_ty, None))).
+
+Definition transfer_tokens' :=
+fun x => transfer_tokens env unit x.1.1 x.1.2 x.2.
+
+Axiom transfer_tokens_inj : injective transfer_tokens'.
+
+Inductive transfer_tokens_proj3_ind :=
+| Transfer_tokens_proj3 p :
+    forall x y z, p (transfer_tokens' (x, y, z)) = Some z
+             -> transfer_tokens_proj3_ind.
+
+Axiom transfer_tokens_proj3 : transfer_tokens_proj3_ind.
+
+Coercion transfer_tokens_proj3_morph
+         (x : transfer_tokens_proj3_ind) :=
+  match x with
+  | Transfer_tokens_proj3 p _ _ _ _ => p
+  end.
+
+Lemma
+data (contract unit)
+
+Lemma refund_refund
+      (xs : seq (data parameter_ty * Datatypes.nat))
+      storage :
+let (res, tt) := compN env crowdfunding xs storage in
+@uniq [eqType of data operation] (seq.map (transfer_tokens_proj3_morph transfer_tokens_proj3) res.1).
+Proof.
+  elim: xs  => //= x xs.
+  move eq: (compN _ _ _ _) => A.
+  case: A eq => [][] /= res storage' []/= eqA IH.
+  rewrite /comp.
+  move eq: (eval_seq env crowdfunding x.2 (x.1, storage', tt)) => B.
+  case: B eq => // [] a.
+  rewrite return_precond eval_seq_precond_correct -eval_seq_precond_correct.
+  case: storage' eqA => [][] raisers refund_table [][] withdrawn funding_start
+                     [] funding_end unconditional_refund_start eqA.
+  case: x => [][y|[|]y] z.
+  + case z5 : (z > 5); last first.
+     move/negP/negP: z5; rewrite -leqNgt => C H.
+     move: H (crowdfunding_fail_contribute env y raisers refund_table funding_start funding_end unconditional_refund_start withdrawn (eq^~ a) C).
+     by rewrite -return_precond => ->.
+    rewrite crowdfunding_correct_contribute //=.
+    case: (map.get _ _ _ _ _) => /= [a0|[]?[]? <-] //.
+    case: (tez.of_Z _) => // a1 /= []?[]? <- //=.
+  + case z7 : (z > 7); last first.
+     move/negP/negP: z7; rewrite -leqNgt => C H.
+     move: H (crowdfunding_fail_withdraw env y raisers refund_table funding_start funding_end unconditional_refund_start withdrawn (eq^~ a) C).
+     by rewrite -return_precond => ->.
+    rewrite crowdfunding_correct_withdraw //=.
+    case=>[]? []? []? []C0 []? [] ? []? <-.
+    rewrite uniq_catC cat_uniq IH /= orbF andbT.
+    move: (f_equal (fun x => x.1.1) eqA) => /= {eqA} eqA.
+    apply/negP => C {IH}.
+    suff: withdrawn = true by rewrite C0.
+    elim: res C xs storage eqA => //= a0 l IH.
+    rewrite (@in_cons [eqType of data operation]).
+    case/orP=> [/eqP <-|{}/IH // IH]; last first.
+     elim => //= x xs IH0 storage.
+     rewrite /comp /=.
+     move eq: (eval_seq _ _ _ _) => B.
+     case: B eq => [e + H|a1].
+      by move: (IH0 storage H).
+     case: a1 => [][]/= ++ [].
+     move=> a1 b H.
+     move: (size_crowdfunding_operations H).
+     case: a1 H => [H ?|a1[]//]; last first.
+      by move=> ?? []? /IH.
+     by move/IH0.
+    case=>//=.
+
+
+     rewrite return_precond.
+
+      case: xs H => //= a1 xs.
+      rewrite /comp /=.
+      move eq: (eval_seq _ _ _ _) => B.
+      case: B eq => [e0 + H|].
+      rewrite H.
+      rewrite /=.
+      move: (IH (x :: xs) storage) => /=.
+      rewrite /comp /= => + C1.
+      rewrite C1 /=.
+      rewrite H.
+     move eqA: (compN env crowdfunding xs storage) => A.
+     case: A eqA => // A [].
+     rewrite /=.
+     rewrite /=.
+     compN env crowdfunding xs storage
+     rewrite /=.
+
+  move eq: (eval_seq env crowdfunding x.2 (x.1, storage', tt)) => B.
+  case: B eq => // [] a.
+  rewrite return_precond eval_seq_precond_correct -eval_seq_precond_correct.
+     move=> xs storage.
+    Set Printing All.
+    case.
+    rewrite
+    IH eq.
+    Set Printing All.
+    rewrite in_cons.
+    case.
+  rewrite /=.
+  ((raisers, refund_table),
+           ((withdrawn, funding_start),
+            (funding_end, unconditional_refund_start)))
+  rewrite /=.
+  Search (_ = Return _).
+
+  rewrite /=.
+  set B :=
+  eval_seq env crowdfunding x.2 (x.1, storage, tt)
+   IH.
+  rewrite /compN.
+  rewrite /=.
+
+  rewrite -/comp.
+  Check foldl.
+  rewrite
+  rewrite /=.
+  move=> storage.
+
+
+all enough_fuel xs ->
+About transfer_tokens.
+Check contract_ None unit eligible_address
+
+Lemma crowdfunding_correct_compN
+      (env : @proto_env (Some (parameter_ty, None)))
+      (xs : seq (data parameter_ty * Datatypes.nat))
+      (raisers : data (set address))
+      (refund_table : data (big_map address mutez))
+      (funding_start : data timestamp)
+      (funding_end : data timestamp)
+      (unconditional_refund_start : data timestamp)
+      (withdrawn : data bool)
+      (psi : stack (pair (list operation) storage_ty ::: [::]) -> Prop) :
+let remove := map.remove address_constant tez.mutez address_compare
+              (compare_eq_iff address) (lt_trans address) (gt_trans address) in
+let get := map.get address_constant tez.mutez address_compare in
+let storage := ((raisers, refund_table),
+                ((withdrawn, funding_start),
+                 (funding_end, unconditional_refund_start))) in
+precond (compN env crowdfunding xs storage) psi <->
+all enough_fuel xs
+/\
+exists y, get eligible_address refund_table = Some y
+/\ geq (now env) unconditional_refund_start
+/\ withdrawn = false
+/\ (exists y0, contract_ None unit eligible_address = Some y0
+   /\ psi ([:: transfer_tokens env unit tt y y0],
+           (raisers, remove eligible_address refund_table,
+           (withdrawn, funding_start, (funding_end, unconditional_refund_start))), tt)).
+Check precond (compN _ crowdfunding _ _).
+Check bijective _.
+Check precond.
+collect_eligible_address
+Variable (xs : seq (data parameter_ty * Datatypes.nat)).
+Check undup xs.
+Check [set x | x \in xs].
+Check finset.
+Check finset (mem (collect_eligible_address _)).
 End crowdfunding.
